theories/stacked_borrows/examples/opt1.v
@@ -1,0 +1,91 @@
+From simuliris.stacked_borrows Require Import proofmode lang.
+Set Default Proof Using "Type".
+
+(** Moving read of mutable reference up across code not using that ref. *)
+
+
+(* Assuming x : &mut i32 *)
+Definition ex1_unopt : ectx :=
+  (λ: "i",
+    (* get related values i*)
+
+    (* init with same new call id on both sides and obtain knowledge that [c] is active: active(c) *)
+    (* c protects { } *)
+
+    (* "x" is the local variable that stores the pointer value "i" *)
+    let: "x" := new_place (&mut int) "i" in
+    (* get a location l and ptr_id pid; (l, Tagged pid) ↦{tk_local} i;
+       get authoritative knowledge of stack: l @s@ [mkItem Unique (Tagged pid) None]
+    *)
+
+    (* retag_place reborrows the pointer value stored in "x" (which is "i"),
+      then updates "x" with the new pointer value.  A [Default] retag is
+      sufficient for this, we don't need the protector. *)
+    retag_place "x" (RefPtr Mutable) int Default #[0];;
+    (* obtain (through source UB) knowledge that i = #[ScPtr li ti], get  li_t ↔h li
+        (l, Tagged pid) ↦{tk_local} ScPtr li ti' for new tag ti'; 
+        get (li, ti') ↦{tk_mut} v0
+
+    *)
+
+    (* The unknown code is represented by a call to an unknown function "f" or
+      "g". *)
+    Call #[ScFnPtr "f"] #[] ;;
+
+    (* Write 42 to the cell pointed to by the pointer in "x" *)
+    *{int} "x" <- #[42] ;;
+    (* just use the permissions we have *)
+
+    Call #[ScFnPtr "g"] #[] ;;
+
+    (* Read the value "v" from the cell pointed to by the pointer in "x" *)
+    let: "v" := Copy *{int} "x" in
+
+    (* Free the local variable *)
+    Free "x" ;;
+
+    (* Finally, return the read value *)
+    "v")%E
+  .
+
+
+Definition ex1_opt : function :=
+  fun: ["i"],
+    let: "x" := new_place (&mut int) "i" in
+    retag_place "x" (RefPtr Mutable) int Default ;;
+    Call #[ScFnPtr "f"] [] ;;
+    (* *x : l, t *)
+    *{int} "x" <- #[42] ;;    (* stack for *x: mkItem Unique t None :: ... *)
+
+    (* TODO: for now, until we change read semantics, directly have 42 without a read *)
+    let: "v" := #[42] in
+    (*let: "v" := Copy *{int} "x" in [> stack for *x : mkItem Unique t None :: .... ?<]*)
+
+    (* Question: 
+        why do we retain knowledge about x here? Note: we are reading asymmetrically from the bijection here.
+        Because: otherwise, we will reach UB in the source at a later point (in > 1 steps).
+        Reasoning: do a case analysis on the shape of the target stack for li.
+        If this is not what we need, use the bijection to transfer this knowledge to the source stack,
+        then claim that we can reach source stuckness after the call. 
+        But reaching source stuckness after the call seems really complicated!
+
+
+        Does this get easier when we set a protector?
+        Yes. 
+    *)
+
+
+    Call #[ScFnPtr "g"] [] ;;
+    Free "x" ;;
+    "v"
+
+
+(* Where do protectors help me?
+
+        c protects { ti' ↦ { li } }       means: there's an item in the stack which is protected by c 
+
+   protectors help when: 
+    * we can use source UB to find out that there's nothing un-poppable above the protector
+    * we can otherwise maintain that the protected item can be used rn for accesses: if access mode is Unique or Shared, then we can use knowledge of the protector to gain knowledge of the full stack!
+          (this is an invariant that needs to be held up by other threads, and thus makes this reasoning possible locally!)
+*)
