theories/stacked_borrows/examples/opt2.v
@@ -1,0 +1,65 @@
+From simuliris.stacked_borrows Require Import proofmode lang.
+Set Default Proof Using "Type".
+
+(** Moving read of shared ref up across code that *may* use that ref. *)
+
+(* Assuming x : & i32 *)
+Definition ex2_unopt : ectx :=
+  λ: "i",
+    let: "c" := InitCall in
+    (* c protects { } *)
+
+    (* "x" is the local variable that stores the pointer value "i" *)
+    let: "x" := new_place (& int) "i" in
+    (* (x, Tagged pid_x) ↦{tk_local} i *)
+
+    (* retag_place reborrows the pointer value stored in "x" (which is "i"),
+      then updates "x" with the new pointer value. A [Default] retag is
+      sufficient for this, we don't need the protector. *)
+    retag_place "x" (RefPtr Immutable) int Default "c";;
+    (* (x, Tagged pid_x) ↦{tk_local} ScPtr l t 
+       (l, Tagged npid) ↦{tk_shr} v
+    *)
+
+    (* The unknown code is represented by a call to an unknown function "f",
+      which does take the pointer value from "x" as an argument. *)
+    Call #[ScFnPtr "f"] (Copy "x") ;;
+    (* need to insert x into the bijection for the call.
+        point: for this to work, we need to retain some knowledge about the value even beyond the bijection.
+        i.e.: retain a fractional points-to!
+
+        (l, Tagged npid) ↦{q, tk_shr} v
+    *)
+
+    (* Read the value "v" from the cell pointed to by the pointer in "x" *)
+    let: "v" := Copy *{int} "x" in
+
+    (* Free the local variable *)
+    Free "x" ;;
+
+    (* Finally, return the read value *)
+    EndCall "c";;
+    "v"
+  .
+
+Definition ex2_opt : ectx :=
+  λ: "i",
+    let: "c" := InitCall in
+    let: "x" := new_place (& int) "i" in
+    retag_place "x" (RefPtr Immutable) int Default "c";;
+    let: "v" := Copy *{int} "x" in
+    (* NOTE: here we have the same problem as in opt1.v: we need to know that the stack has not changed. 
+        moreover: might need to keep track of the type/type size somewhere?*)
+    Call #[ScFnPtr "f"] (Copy "x") ;;
+    Free "x" ;;
+    EndCall "c";;
+    "v"
+  .
+
+
+(* NOTE regarding allocation size: just weaken that to say that it either has a size or has been deallocated.
+  Then we should be able to make that token persistent. 
+  (we can rule out the "deallocated" case with a pointsto, if needed) 
+*)
+
+
