theories/stacked_borrows/examples/opt2_down.v
@@ -1,0 +1,48 @@
+From simuliris.stacked_borrows Require Import proofmode lang.
+Set Default Proof Using "Type".
+
+(** Moving a read of a shared reference down across code that *may* use that ref. *)
+
+(* Assuming x : & i32 *)
+Definition ex2_down_unopt : ectx :=
+  λ: "i",
+    let: "c" := InitCall in
+    (* "x" is the local variable that stores the pointer value "i" *)
+    let: "x" := new_place (& int) "i" in
+
+    (* retag_place reborrows the pointer value stored in "x" (which is "i"),
+      then updates "x" with the new pointer value. This relies on protectors,
+      hence [FnEntry]. *)
+    retag_place "x" (RefPtr Immutable) int FnEntry "c";;
+
+    (* Read the value "v" from the cell pointed to by the pointer in "x" *)
+    let: "v" := Copy *{int} "x" in
+
+    (* The unknown code is represented by a call to an unknown function "f",
+      which does take the pointer value from "x" as an argument. *)
+    Call #[ScFnPtr "f"] (Copy "x") ;;
+
+    (* Free the local variable *)
+    Free "x" ;;
+
+    (* Finally, return the read value *)
+    EndCall "c";;
+    "v"
+  .
+
+Definition ex2_down_opt : ectx :=
+  λ: "i",
+    let: "c" := InitCall in
+    let: "x" := new_place (& int) "i" in
+    retag_place "x" (RefPtr Immutable) int FnEntry "c";;
+    Call #[ScFnPtr "f"] (Copy "x") ;;
+    let: "v" := Copy *{int} "x" in
+    (* need to make sure that we are reading the same value! -- so take the same strategy of keeping a fraction outside.
+      to be able to use that fraction, need to use the protector.
+    *)
+    Free "x" ;;
+    EndCall "c";;
+    "v"
+  .
+
+
