theories/stacked_borrows/examples/opt3.v
@@ -1,0 +1,52 @@
+From simuliris.stacked_borrows Require Import proofmode lang.
+Set Default Proof Using "Type".
+
+(** Moving a write to a mutable reference up across unknown code. *)
+
+(* Assuming x : &mut i32 *)
+Definition ex3_unopt : ectx :=
+  λ: "i",
+    let: "c" := InitCall in
+    (* "x" is the local variable that stores the pointer value "i" *)
+    let: "x" := new_place (&mut int) "i" in
+
+    (* retag_place reborrows the pointer value stored in "x" (which is "i"),
+      then updates "x" with the new pointer value. This relies on protectors,
+      hence [FnEntry]. *)
+    retag_place "x" (RefPtr Mutable) int FnEntry "c";;
+
+    (* Write 42 to the cell pointed to by the pointer in "x" *)
+    *{int} "x" <- #[42] ;;
+    (* Challenge here: the bijection is running out of sync! 
+        Point: the entry in the bijection should effectively be disabled, due to the unique tag + protector.
+
+        the stack shape assertion is in the bijection. Point: it doesn't necessarily grant access. 
+       (remember, the pointsto assertions are conditional -- the bijection does not contain the knowledge needed to use that; that has to be kept externally).
+    *)
+
+    (* The unknown code is represented by a call to an unknown function "f" *)
+    let: "v" := Call #[ScFnPtr "f"] #[] in
+
+    (* Write 13 to the cell pointed to by the pointer in "x" *)
+    *{int} "x" <- #[13] ;;
+
+    (* Free the local variable *)
+    Free "x" ;;
+
+    (* Finally, return the value *)
+    EndCall "c";;
+    "v"
+  .
+
+Definition ex3_opt : ectx :=
+  λ: "i",
+    let: "c" := InitCall in
+    let: "x" := new_place (&mut int) "i" in
+    retag_place "x" (RefPtr Mutable) int FnEntry "c";;
+    *{int} "x" <- #[13] ;;
+    let: "v" := Call #[ScFnPtr "f"] #[] in
+    Free "x" ;;
+    EndCall "c";;
+    "v"
+  .
+
